[isasat] more type fixes

Weidenbach_Book/IsaSAT/IsaSAT_LLVM.thy
@@ -13,20 +13,18 @@ hide_const (open)IICF_Multiset.mset_rel
 chapter \<open>Code of Full IsaSAT\<close>
 
 abbreviation  model_stat_assn where
-  \<open>model_stat_assn \<equiv> bool1_assn \<times>\<^sub>a (arl64_assn unat_lit_assn) \<times>\<^sub>a stats_int_assn\<close>
+  \<open>model_stat_assn \<equiv> bool1_assn \<times>\<^sub>a (arl64_assn unat_lit_assn) \<times>\<^sub>a isasat_stats_assn\<close>
 
 abbreviation model_stat_assn\<^sub>0 ::
     \<open>bool \<times>
      nat literal list \<times>
-     64 word \<times>
-     64 word \<times> 64 word \<times> 64 word \<times> 64 word \<times> 64 word \<times> 64 word \<times> 64 word\<times> 64 word \<times>  64 word\<times> 64 word\<times>  64 word\<times> 64 word \<times> ema
+     isasat_stats
      \<Rightarrow> 1 word \<times>
        (64 word \<times> 64 word \<times> 32 word ptr) \<times>
-       64 word \<times>
-       64 word \<times> 64 word \<times> 64 word \<times> 64 word \<times> 64 word \<times> 64 word \<times> 64 word\<times> 64 word \<times> 64 word\<times> 64 word\<times>  64 word\<times> 64 word\<times> ema
+       _
        \<Rightarrow> llvm_amemory \<Rightarrow> bool\<close>
 where
-  \<open>model_stat_assn\<^sub>0 \<equiv> bool1_assn \<times>\<^sub>a (al_assn unat_lit_assn) \<times>\<^sub>a stats_int_assn\<close>
+  \<open>model_stat_assn\<^sub>0 \<equiv> bool1_assn \<times>\<^sub>a (al_assn unat_lit_assn) \<times>\<^sub>a isasat_stats_assn\<close>
 
 abbreviation lits_with_max_assn :: \<open>nat multiset
      \<Rightarrow> (64 word \<times> 64 word \<times> 32 word ptr) \<times> 32 word \<Rightarrow> llvm_amemory \<Rightarrow> bool\<close> where
@@ -85,7 +83,7 @@ lemma extract_model_of_state_stat_alt_def:
          mop_free cach; mop_free lbd; mop_free outl; mop_free heur;
          mop_free vdom; mop_free opts;
          mop_free old_arena; mop_free lcount; mop_free occs;
-        RETURN (False, M, get_content stats)
+        RETURN (False, M, stats)
      })\<close>
   by (auto simp: extract_model_of_state_stat_def mop_free_def print_trail2_def split_trail_def
     intro!: ext split: isasat_int_splits)
@@ -110,7 +108,7 @@ lemma extract_state_stat_alt_def:
          mop_free cach; mop_free lbd; mop_free outl; mop_free heur;
          mop_free vdom; mop_free opts;
          mop_free old_arena; mop_free lcount;  mop_free occs;
-        RETURN (True, [], get_content stats)})\<close>
+        RETURN (True, [], stats)})\<close>
   by (auto simp: extract_state_stat_def mop_free_def split: isasat_int_splits intro!: ext)
 
 sepref_def extract_state_stat
@@ -412,6 +410,117 @@ sepref_def print_binary_red_removed_impl
 abbreviation (input) C_bool_to_bool :: \<open>8 word \<Rightarrow> bool\<close> where
   \<open>C_bool_to_bool g \<equiv> g \<noteq> 0\<close>
 
+
+definition stats_decisions :: \<open>isasat_stats \<Rightarrow> 64 word\<close> where
+  \<open>stats_decisions = Search_Stats_decisions o get_search_stats\<close>
+
+definition stats_irred :: \<open>isasat_stats \<Rightarrow> 64 word\<close> where
+  \<open>stats_irred = Search_Stats_irred o get_search_stats\<close>
+
+definition Binary_Stats_rounds :: \<open>inprocessing_binary_stats \<Rightarrow> 64 word\<close> where
+  \<open>Binary_Stats_rounds = (\<lambda>(rounds, units, removed). rounds)\<close>
+
+definition stats_binary_rounds :: \<open>isasat_stats \<Rightarrow> 64 word\<close> where
+  \<open>stats_binary_rounds = Binary_Stats_rounds o get_binary_stats\<close>
+
+definition Binary_Stats_units :: \<open>inprocessing_binary_stats \<Rightarrow> 64 word\<close> where
+  \<open>Binary_Stats_units = (\<lambda>(units, units, removed). units)\<close>
+
+definition stats_binary_units :: \<open>isasat_stats \<Rightarrow> 64 word\<close> where
+  \<open>stats_binary_units = Binary_Stats_units o get_binary_stats\<close>
+
+definition Binary_Stats_removed :: \<open>inprocessing_binary_stats \<Rightarrow> 64 word\<close> where
+  \<open>Binary_Stats_removed = (\<lambda>(removed, units, removed). removed)\<close>
+
+definition stats_binary_removed :: \<open>isasat_stats \<Rightarrow> 64 word\<close> where
+  \<open>stats_binary_removed = Binary_Stats_removed o get_binary_stats\<close>
+
+definition Pure_Lits_Stats_removed :: \<open>inprocessing_pure_lits_stats \<Rightarrow> 64 word\<close> where
+  \<open>Pure_Lits_Stats_removed = (\<lambda>(removed, removed). removed)\<close>
+
+definition stats_pure_lits_removed :: \<open>isasat_stats \<Rightarrow> 64 word\<close> where
+  \<open>stats_pure_lits_removed = Pure_Lits_Stats_removed o get_pure_lits_stats\<close>
+
+definition Pure_Lits_Stats_rounds :: \<open>inprocessing_pure_lits_stats \<Rightarrow> 64 word\<close> where
+  \<open>Pure_Lits_Stats_rounds = (\<lambda>(rounds, rounds). rounds)\<close> 
+
+definition stats_pure_lits_rounds :: \<open>isasat_stats \<Rightarrow> 64 word\<close> where
+  \<open>stats_pure_lits_rounds = Pure_Lits_Stats_rounds o get_pure_lits_stats\<close>
+
+sepref_def Search_Stats_decisions_impl
+  is \<open>RETURN o Search_Stats_decisions\<close>
+  :: \<open>search_stats_assn\<^sup>k \<rightarrow>\<^sub>a word64_assn\<close>
+  unfolding search_stats_assn_def Search_Stats_decisions_def
+  by sepref
+
+sepref_def Search_Stats_irred_impl
+  is \<open>RETURN o Search_Stats_irred\<close>
+  :: \<open>search_stats_assn\<^sup>k \<rightarrow>\<^sub>a word64_assn\<close>
+  unfolding search_stats_assn_def Search_Stats_irred_def
+  by sepref
+
+
+sepref_def Binary_stats_rounds_impl
+  is \<open>RETURN o Binary_Stats_rounds\<close>
+  :: \<open>binary_stats_assn\<^sup>k \<rightarrow>\<^sub>a word64_assn\<close>
+  unfolding binary_stats_assn_def Binary_Stats_rounds_def
+  by sepref
+
+sepref_def Binary_stats_units_impl
+  is \<open>RETURN o Binary_Stats_units\<close>
+  :: \<open>binary_stats_assn\<^sup>k \<rightarrow>\<^sub>a word64_assn\<close>
+  unfolding binary_stats_assn_def Binary_Stats_units_def
+  by sepref
+
+sepref_def Binary_stats_removed_impl
+  is \<open>RETURN o Binary_Stats_removed\<close>
+  :: \<open>binary_stats_assn\<^sup>k \<rightarrow>\<^sub>a word64_assn\<close>
+  unfolding binary_stats_assn_def Binary_Stats_removed_def
+  by sepref
+
+sepref_def Pure_Lits_Stats_removed_impl
+  is \<open>RETURN o Pure_Lits_Stats_removed\<close>
+  :: \<open>pure_lits_stats_assn\<^sup>k \<rightarrow>\<^sub>a word64_assn\<close>
+  unfolding pure_lits_stats_assn_def Pure_Lits_Stats_removed_def
+  by sepref
+
+sepref_def Pure_Lits_Stats_removed_rounds_impl
+  is \<open>RETURN o Pure_Lits_Stats_rounds\<close>
+  :: \<open>pure_lits_stats_assn\<^sup>k \<rightarrow>\<^sub>a word64_assn\<close>
+  unfolding pure_lits_stats_assn_def Pure_Lits_Stats_rounds_def
+  by sepref
+
+sepref_register Search_Stats_decisions Pure_Lits_Stats_rounds Pure_Lits_Stats_removed
+  Binary_Stats_removed Binary_Stats_rounds Binary_Stats_units
+sepref_def stats_decisions_impl
+  is \<open>RETURN o stats_decisions\<close> :: \<open>isasat_stats_assn\<^sup>k \<rightarrow>\<^sub>a word64_assn\<close>
+ unfolding stats_decisions_def stats_code_unfold by sepref
+
+sepref_def stats_irred_impl
+  is \<open>RETURN o stats_irred\<close> :: \<open>isasat_stats_assn\<^sup>k \<rightarrow>\<^sub>a word64_assn\<close>
+ unfolding stats_irred_def stats_code_unfold by sepref
+
+sepref_def stats_binary_units_impl
+  is \<open>RETURN o stats_binary_units\<close> :: \<open>isasat_stats_assn\<^sup>k \<rightarrow>\<^sub>a word64_assn\<close>
+ unfolding stats_binary_units_def stats_code_unfold by sepref
+
+sepref_def stats_binary_removed_impl
+  is \<open>RETURN o stats_binary_removed\<close> :: \<open>isasat_stats_assn\<^sup>k \<rightarrow>\<^sub>a word64_assn\<close>
+ unfolding stats_binary_removed_def stats_code_unfold by sepref
+sepref_def stats_binary_rounds_impl
+  is \<open>RETURN o stats_binary_rounds\<close> :: \<open>isasat_stats_assn\<^sup>k \<rightarrow>\<^sub>a word64_assn\<close>
+ unfolding stats_binary_rounds_def stats_code_unfold by sepref
+
+sepref_def stats_pure_lits_rounds_impl
+  is \<open>RETURN o stats_pure_lits_rounds\<close> :: \<open>isasat_stats_assn\<^sup>k \<rightarrow>\<^sub>a word64_assn\<close>
+ unfolding stats_pure_lits_rounds_def stats_code_unfold by sepref
+
+sepref_def stats_pure_lits_removed_impl
+  is \<open>RETURN o stats_pure_lits_removed\<close> :: \<open>isasat_stats_assn\<^sup>k \<rightarrow>\<^sub>a word64_assn\<close>
+ unfolding stats_pure_lits_removed_def stats_code_unfold by sepref
+
+
+
 definition IsaSAT_bounded_heur_wrapper :: \<open>8 word \<Rightarrow> 8 word \<Rightarrow> 8 word \<Rightarrow> 64 word \<Rightarrow> 64 word \<Rightarrow> nat \<Rightarrow>
   8 word \<Rightarrow> 64 word \<Rightarrow> 64 word \<Rightarrow> 64 word \<Rightarrow> _ \<Rightarrow> (nat) nres\<close>where
   \<open>IsaSAT_bounded_heur_wrapper red res unbdd mini res1 res2 target_option fema sema units C = do {
@@ -419,19 +528,19 @@ definition IsaSAT_bounded_heur_wrapper :: \<open>8 word \<Rightarrow> 8 word \<R
          (C_bool_to_bool unbdd) mini res1 res2
          (if target_option = 2 then 2 else if target_option = 0 then 0 else 1)
          fema sema units;
-      (b, (b', (_, propa, confl, dec, res, reduction, uset, gcs, _, irred_clss, binary_unit, binary_red_removed, purelit_elim, purelit_rounds, d))) \<leftarrow> IsaSAT_bounded_heur (opts) C;
-      let _ = print_propa propa;
-      let _ = print_confl confl;
-      let _ = print_dec dec;
-      let _ = print_res res;
-      let _ = print_lres reduction;
-      let _ = print_uset uset;
-      let _ = print_gcs gcs;
-      let _ = print_irred_clss irred_clss;
-      let _ = print_binary_unit binary_unit;
-      let _ = print_binary_red_removed binary_red_removed;
-      let _ = print_purelit_elim purelit_elim;
-      let _ = print_purelit_rounds purelit_rounds;
+      (b, (b', _, stats)) \<leftarrow> IsaSAT_bounded_heur (opts) C;
+      let _ = print_propa (stats_propagations stats);
+      let _ = print_confl (stats_conflicts stats);
+      let _ = print_dec (stats_decisions stats);
+      let _ = print_res (stats_restarts stats);
+      let _ = print_lres (stats_reductions stats);
+      let _ = print_uset (stats_fixed stats);
+      let _ = print_gcs (stats_gcs stats);
+      let _ = print_irred_clss (stats_irred stats);
+      let _ = print_binary_unit (stats_binary_units stats);
+      let _ = print_binary_red_removed (stats_binary_removed stats);
+      let _ = print_purelit_elim (stats_pure_lits_removed stats);
+      let _ = print_purelit_rounds (stats_pure_lits_rounds stats);
       RETURN ((if b then 2 else 0) + (if b' then 1 else 0))
   }\<close>
 
