Weidenbach_Book/IsaSAT/IsaSAT_Rephase_State_LLVM.thy
@@ -89,3 +89,5 @@ export_llvm rephase_heur_st_impl
   save_phase_heur_st
 
 end
+
+end
